update

data_struct.v
@@ -7,16 +7,15 @@ Require Import flows.flows.
 Require Import iris_ora.algebra.gmap.
 Require Import iris_ora.logic.own.
 Require Import iris_ora.algebra.ext_order.
+Require Import iris_ora.algebra.frac_auth.
 Require Import VST.floyd.proofauto.
 Require Import VST.atomics.general_locks.
-Require Import Coq.Sets.Ensembles. 
-Require Import bst.puretree.
-Require Import bst.giveup_template.
 Require Import VST.floyd.library.
 Require Import VST.atomics.verif_lock_atomic.
-From iris_ora.algebra Require Import frac_auth.
-Require Import bst.flows_ora.
-Require Import bst.keyset_ra_ora.
+Require Import templ.puretree.
+Require Import templ.giveup_template.
+Require Import templ.flows_ora.
+Require Import templ.keyset_ra_ora.
 
 Definition Key := Z.
 
@@ -36,23 +35,7 @@ Section Give_Up_Cameras.
   Proof. solve_inG. Qed.
 
   (* RA for authoritative sets of nodes *)
-  (* Definition gset1 := gmap K unit. *)
-  (*
-  Canonical Structure gsetR A `{Countable A} := gmapR A unit.
-  Canonical Structure gsetUR A `{Countable A} := gmapUR A unit.
-  Lemma gst A `{Countable A} n (x y : gsetUR A): ✓{n} y → x ≼ₒ{n} y → x ≼{n} y.
-  Proof.
-    intros Hv Hxy.
-    rewrite lookup_includedN; intros i.
-    specialize (Hv i); specialize (Hxy i); rewrite option_includedN.
-    destruct (x !! i) as [a|] eqn: Hx; last by auto.
-    rewrite Hx in Hxy |- *.
-    destruct (_ !! _) as [b|]; last done;
-    right; eexists _, _; split; first done.
-    split; first done; auto.
-  Qed.
-*)
-  Locate authR.
+  
   Canonical Structure gset_authR A `{Countable A} := inclR(iris.algebra.auth.authR(gsetR A)).
 
   Class nodesetG Σ := NodesetG { nodeset_inG :> inG Σ (gset_authR Node ) }.
@@ -95,36 +78,36 @@ Proof.
   unfold Inhabitant; apply F.
 Defined.
 
+Definition pointer_of (n : Node) :=  fst n.
+Definition lock_of (n : Node) := fst (snd n).
+Definition node_of (n : Node) := snd (snd n).
+
 
 Section NodeRep.
-  Context `{!VSTGS unit Σ, !flowintG Σ, !nodesetG Σ, !keysetG Σ }.
-
-  Definition inFP (γ_f: gname) (n : Node) : mpred :=
+Context `{!VSTGS unit Σ, !flowintG Σ, !nodesetG Σ, !keysetG Σ }.
+Definition inFP (γ_f: gname) (n : Node) : mpred :=
     ∃ (N: gset Node),
       (own (inG0 := nodeset_inG)) γ_f (◯ N : gset_authR _) ∧ ⌜n ∈ N⌝.
 
-  Class NodeRep : Type := {
+Class NodeRep : Type := {
       node : Node → @multiset_flowint_ur Key _ _ → gset Key → mpred;
       node_sep_star: ∀ n I_n I_n' C C', node n I_n C ∗ node n I_n' C' -∗ False;
-      (*node_rep_R_valid_pointer: forall n I_n C, node n I_n C -∗ valid_pointer n;
-      node_rep_R_pointer_null: forall n I_n C, node n I_n C -∗ ⌜is_pointer_or_null n⌝; *)
+      node_rep_R_valid_pointer: forall n I_n C, node n I_n C -∗ valid_pointer (pointer_of n);
+      node_rep_R_pointer_null: forall n I_n C, node n I_n C -∗ ⌜is_pointer_or_null (pointer_of n)⌝;
       node_size: nat;
-  }.
+}.
    
-  Global Instance inFP_persistent γ_f n: Persistent (inFP γ_f n).
-  Proof.
-    apply bi.exist_persistent.
-    intros.
-    apply bi.and_persistent; try apply _.
-    apply own_core_persistent.
-    Locate auth_frag_core_id.
-    apply (iris.algebra.auth.auth_frag_core_id _ ).
-    apply _.
-  Qed.
+Global Instance inFP_persistent γ_f n: Persistent (inFP γ_f n).
+Proof.
+  apply bi.exist_persistent.
+  intros.
+  apply bi.and_persistent; try apply _.
+  apply own_core_persistent.
+  apply (iris.algebra.auth.auth_frag_core_id _ ).
+  apply _.
+Qed.
 
 End NodeRep.
-
-Check NodeRep.
 
 #[export] Instance CompSpecs : compspecs. make_compspecs prog. Defined.
 Definition Vprog : varspecs.  mk_varspecs prog. Defined.
@@ -138,15 +121,12 @@ Section give_up.
   Definition t_struct_nodeds := Tstruct _node noattr.
   Definition t_struct_pn := Tstruct _pn noattr.
 
-  (*
-    typedef struct node_t {node *t; lock_t lock; int min; int max; } node_t;
-    typedef struct node {int key; void *value; void *left, *right;} node;
-   *)
-  Print Node.
+  (* struct node_t {node *t; lock_t lock; int min; int max; } node_t;
+    struct node {int key; void *value; void *left, *right;} node; *)
 
   Definition node_rep γ_f (pn n lock: val) (min max : number) I_n C :=
     ⌜repable_signed (number2Z min) ∧ repable_signed (number2Z max) /\
-      is_pointer_or_null n /\ is_pointer_or_null lock⌝ ∧ 
+      is_pointer_or_null n /\ is_pointer_or_null lock⌝ ∧
       field_at Ews (t_struct_node) [StructField _t] n pn ∗ (* pn ->n*) 
       field_at Ews (t_struct_node) [StructField _min] (vint (number2Z (min))) pn ∗ (*pn -> min*)
       field_at Ews (t_struct_node) [StructField _max] (vint (number2Z (max))) pn ∗ (*pn -> max*) 
@@ -154,20 +134,16 @@ Section give_up.
       node (pn, (lock, n)) I_n C.
 
 
-  Definition nodePred γ_I γ_k n (In : @multiset_flowint_ur Key _ _ ) Cn  : mpred :=
+  Definition nodePred γ_I γ_k n (In : @multiset_flowint_ur Key _ _ ) Cn :=
    node n In Cn ∗ own γ_k (◯ prod (keyset _ _ Key In n, Cn): keyset_authR Key) ∗
      own γ_I (◯ In) ∗ ⌜dom In = {[n]}⌝.
 
-  Check gset.
 
-  Definition ltree (p lock : val) R:=
+  Definition ltree (p lock : val) R :=
   ∃ lsh, ⌜field_compatible t_struct_node nil p /\ readable_share lsh⌝ ∧
   (field_at lsh t_struct_node [StructField _lock] lock p ∗ inv_for_lock lock R).
 
-  Check inv_for_lock _ .
-
-  Definition lock_of (n : Node) := fst (snd n).
-
+  
   Definition node_lock_inv_pred  gp node := my_half gp 1 (to_agree node) .
   
   Definition globalGhost
@@ -175,78 +151,18 @@ Section give_up.
     own γ_I (● I) ∗ ⌜globalinv _ _ Key r I⌝ ∗
       own γ_k (● prod (KS, C): keyset_authR Key) ∗ own (inG0 := nodeset_inG) γ_f (● (dom I)).
 
-  Set Printing Implicit.
-  Print multiset_flowint_ur.
-  Print flowintUR .
-  Locate flowintT.
-  (* (gset Node)  *)
-  
-  Lemma node_exist_in_tree (* `{Dom multiset_flowint_ur multiset_flowint_ur} *)
-    (γ_f: gname) (n : (val * val * Node)) (I: @multiset_flowint_ur Key _ _):
-    inFP γ_f n ∗ own γ_f (● (dom I)) ⊢ ⌜snd n ∈ I⌝.
+  Lemma node_exist_in_tree γ_f n (I: @multiset_flowint_ur Key _ _):
+    inFP γ_f n ∗ own (inG0 := nodeset_inG) γ_f (● (dom I)) ⊢ ⌜n ∈ dom I⌝.
   Proof.
     intros; iIntros "(#Hfp & Hown)".
     unfold inFP.
     iDestruct "Hfp" as (n1) "[Hown1 %H1]".
-    iDestruct (own_valid_2 _  with "Hown Hown1") as "H1".
-    destruct n.
-    simpl.
-    Check excl_auth_agree.
-    
-  Admitted.
-
-  Check inv_for_lock _ .
-  Check lock_inv.
-
-  Definition test (R: iPropO Σ) (lock : val) i g : mpred : cinv i g (inv_for_lock lock R) .
-
-  
-  
-
-  Definition node_lock_inv_pred g p gp node := my_half gp Tsh node * node_rep p g gp node.
-  
-  
-
-  
-  
+    iDestruct (own_valid_2 _  with "Hown Hown1") as %Hown.
+    rewrite auth_both_valid_discrete in Hown.
+    destruct Hown as (Hin & _).
+    iPureIntro.
+    set_solver.
+  Qed.
 
 
-(** Definitions of cameras used in the template verification *)
-
-
-
-#[export] Instance pointer_lock : Ghost := discrete_PCM (val * val * range).
-Definition ghost_info : Type := (key * val * (list val))%type.
-
-(* This allows the range to be outdated while the ghost_info may be present or absent. *)
-#[export] Instance node_ghost : Ghost := prod_PCM pointer_lock (exclusive_PCM (option ghost_info)).
-Notation node_info := (@G node_ghost).
-
-Definition in_tree (g: gname) (g1 : gname) (pn: val) (lock: val):=
-      ghost_snap (P := gmap_ghost (K := gname)(A := discrete_PCM (val * val)) )
-        ({[g1 := (pn, lock)]}) g.
-
-Lemma in_tree_equiv g g_in p1 p2 lk1 lk2:
-  in_tree g g_in p1 lk1 * in_tree g g_in p2 lk2 |-- !!((p1 = p2) /\ (lk1 = lk2)) .
-Proof.
-  iIntros "H".
-  iPoseProof(ghost_snap_join' with "H") as (v') "(%H & _)".
-  iPureIntro.
-  specialize (H g_in).
-  rewrite ! lookup_insert in H.
-  inversion H; subst; inversion H3; inversion H0; auto.
-Qed.
-
-Lemma in_tree_duplicate g gin pn lock:
-  in_tree g gin pn lock |-- in_tree g gin pn lock * in_tree g gin pn lock.
-Proof. by rewrite - bi.persistent_sep_dup. Qed.
-
-Section NodeRep.
-  Class NodeRep : Type := {
-      node_rep_R : val -> option (option ghost_info) -> gname -> mpred;
-      node_rep_R_valid_pointer: forall tp g_in g, node_rep_R tp g_in g |-- valid_pointer tp;
-      node_rep_R_pointer_null: forall tp g_in g, node_rep_R tp g_in g |-- !! is_pointer_or_null tp;
-      node_size: nat;
-      node_null: forall g_info, node_rep_R nullval g_info = !!(g_info = Some None) && seplog.emp;
-  }.
-End NodeRep.
+End give_up.
